\noindent The system can represented in state space as

\begin{equation}
\begin{array}{c}
\dot{x}(t) = \mbox{A}x(t) + \mbox{B}u(t) \\
y(t) = \mbox{C}x(t) + \mbox{D}u(t)
\end{array}
\end{equation}

\begin{equation}\label{eq:ssTR}
\begin{array}{llllll}

x(t)
&

 =

&

 
\left[
\begin{array}{l}
\dot{\theta_a} 	\\ 
\theta_a		\\
\dot{\theta_L}	\\
\theta_L
\end{array}
\right]



&


,


&

u(t) =T(t)


\end{array}
\end{equation}


and


\begin{equation}
\begin{array}{ccc}
\mbox{A}
&
=
&

\left[
\begin{array}{cccc}
\frac{-(B_a+B_c)}{J_a}   	& \frac{-K_c}{J_a}   	& \frac{B_c}{J_a}   		&	\frac{K_c}{J_a} \\
1 					& 0				& 0					&	0			\\
\frac{B_c}{J_L}			& \frac{K_c}{J_L}	& \frac{-(B_c+B_L)}{J_L}	& 	\frac{-K_c}{J_L} \\
0					& 0				& 0					&	1		
\end{array}

\right]


\end{array}
\end{equation}



\begin{equation}
\mbox{B} = 
\left[
\begin{array}{cccc}
J^{-1}_a 	&
0		&
0		&
0
\end{array}
\right]^{-1}
\end{equation}

\begin{equation}
\begin{array}{ccc}
\mbox{C}
=
\left[
\begin{array}{cccc}
0 	&	1	&	0	&	0
\end{array}
\right]
&
,
&
\mbox{D} = 0
\end{array}
\end{equation}
